theories/foo.v
@@ -1,0 +1,939 @@
+(*
+ * Copyright (c) Meta Platforms, Inc. and affiliates.
+ *
+ * This source code is licensed under the MIT license found in the
+ * LICENSE file in the root directory of this source tree.
+ *)
+From stdpp Require Import base strings gmap stringmap fin_maps.
+
+From iris.proofmode Require Import tactics.
+From iris.base_logic.lib Require Import iprop own wsat.
+From iris.algebra.lib Require Import gmap_view.
+
+From shack Require Import lang progdef subtype ok typing.
+From shack Require Import eval heap modality interp.
+
+
+(*
+<<__SupportDynamicType>>
+   class C {
+     private Bool $prop = new I();
+
+     <<__SupportDynamicType>>
+     private function set(Bool $vi):void {
+       $this->prop = $vi;
+     }
+
+     public function breakit(dynamic $d):void {
+       $d->set(3);
+     }
+
+     public function getFst(): bool {
+       return $this->prop;
+     }
+   }
+
+   <<__EntryPoint>>
+   function main():void {
+     $c = new C();
+     $c->breakit($c);
+     $x = $c->getFst();
+     var_dump($x);
+   }
+*)
+Definition Set_ := {|
+  methodargs := {[ "$vi" := BoolT ]};
+  methodrettype := NullT;
+  methodbody := SetC ThisE "$prop" (VarE "$vi");
+  methodret := NullE;
+  methodvisibility := Private;
+|}.
+
+Definition BreakIt := {|
+  methodargs := {[ "$d" := DynamicT ]};
+  methodrettype := NullT;
+  methodbody := CallC "$_" (VarE "$d") "set" {[ "$vi" := IntE 3 ]};
+  methodret := NullE;
+  methodvisibility := Public;
+|}.
+
+Definition Get_ := {|
+  methodargs := ∅;
+  methodrettype := BoolT;
+  methodbody := GetC "$ret" ThisE "$prop";
+  methodret := VarE "$ret";
+  methodvisibility := Public;
+|}.
+
+Definition C := {|
+  superclass := None;
+  generics := [];
+  constraints := [];
+  classfields := {["$prop" := (Private, BoolT) ]};
+  classmethods := {["set" := Set_; "get" := Get_; "breakit" := BreakIt]};
+|}.
+
+Definition main_fun := {|
+  methodargs := ∅;
+  methodrettype := NullT;
+  methodbody :=
+  SeqC
+    (NewC "$c" "C" None {[ "$prop" := BoolE false ]})
+    (SeqC 
+    (CallC "$0" (VarE "$c") "breakit" {[ "$d" := UpcastE (VarE "$c") DynamicT ]})
+    (CallC "$1" (VarE "$c") "get" ∅));
+  methodret := NullE;
+  methodvisibility := Public;
+|}.
+
+Definition M := {|
+  superclass := None;
+  generics := [];
+  constraints := [];
+  classfields := ∅;
+  classmethods := {[ "main" := main_fun ]};
+|}.
+
+Local Instance PDC : ProgDefContext := {
+  pdefs := {[ "C" := C; "M" := M ]};
+}.
+
+Lemma pacc : ∀ c : tag, Acc (λ x y : tag, extends y x) c.
+Proof.
+  move => c.
+  destruct (String.eqb c "C") eqn:heq0.
+  { apply String.eqb_eq in heq0 as ->.
+    constructor => t hext.
+    inv hext.
+    rewrite lookup_insert in H; case: H => H; subst.
+    rewrite /C /= in H0.
+    discriminate.
+  }
+  apply String.eqb_neq in heq0.
+  destruct (String.eqb c "M") eqn:heq1.
+  { apply String.eqb_eq in heq1 as ->.
+    constructor => t hext.
+    inv hext.
+    rewrite lookup_insert_ne in H; last done.
+    rewrite lookup_insert in H; case: H => H; subst.
+    rewrite /M /= in H0.
+    discriminate.
+  }
+  apply String.eqb_neq in heq1.
+  constructor => t hext; exfalso.
+  inv hext.
+  by repeat (rewrite lookup_insert_ne // in H).
+Qed.
+
+Local Instance PDA : ProgDefAcc  := { pacc := pacc }.
+
+(* This is where we encode the <<SDT>> attribute *)
+Definition CSDT : list constraint := [].
+
+Definition CFalse : constraint := (IntT, BoolT).
+
+Definition SDT (t: tag)  : list constraint :=
+  if String.eqb t "C" then CSDT else
+  [CFalse]
+.
+
+Definition SDT_M (t: tag) (m: string) : list constraint :=
+  if String.eqb t "C" && String.eqb m "set" then CSDT else
+  if String.eqb t "C" && String.eqb m "get" then CSDT else
+  if String.eqb t "C" && String.eqb m "breakit" then CSDT else
+  [CFalse]
+.
+
+Local Instance SDTCC : SDTClassConstraints := {
+  Δsdt := SDT;
+  Δsdt_m := SDT_M;
+}.
+
+Local Instance SDTCS : SDTClassSpec.
+Proof.
+  split.
+  - rewrite /Δsdt /= /SDT => A k c.
+    destruct (A =? "C")%string; first done.
+    destruct (A =? "M")%string.
+    { rewrite list_lookup_singleton.
+      case : k => [ | k] //=.
+      case => <-; by repeat constructor.
+    }
+    rewrite list_lookup_singleton.
+    case : k => [ | k] //=.
+    case => <-; by repeat constructor.
+  - rewrite /Δsdt_m /= /SDT_M => A m k c.
+    destruct (A =? "C")%string eqn:h0 => /=.
+    { destruct (m =? "set")%string => /=; first done.
+      destruct (m =? "get")%string => /=; first done.
+      destruct (m =? "breakit")%string => /=; first done.
+      rewrite list_lookup_singleton.
+      case : k => [ | k] //=.
+      case => <-; by repeat constructor.
+    }
+    rewrite list_lookup_singleton_Some => [[? <-]].
+    by repeat constructor.
+  - rewrite /Δsdt /= /SDT => A adef k c.
+    rewrite lookup_insert_Some => [[[<- <-] | ]] /=; first done.
+    case => ?; rewrite lookup_singleton_Some => [[<- <-]] /=.
+    rewrite list_lookup_singleton_Some => [[? <-]].
+    by repeat constructor.
+  - rewrite /Δsdt_m /= /SDT_M => A m adef k c.
+    rewrite lookup_insert_Some => [[[<- <-] | ]] /=.
+    { destruct (m =? "set")%string; first done.
+      destruct (m =? "get")%string; first done.
+      destruct (m =? "breakit")%string; first done.
+      case : k => [ | k] //=.
+      case => <-; by repeat constructor.
+    }
+    case => ?; rewrite lookup_singleton_Some => [[<- <-]] /=.
+    rewrite list_lookup_singleton_Some => [[<- <-]].
+    by repeat constructor.
+Qed.
+
+Local Instance SDTCVS : SDTClassVarianceSpec.
+Proof.
+  split.
+  move => Δ kd A adef σ0 σ1 hadef hσ.
+  move => i c0 h.
+  assert (hl0: length adef.(generics) = length σ0) by by eapply length_subtype_targs_v0.
+  assert (hl1: length σ0 = length σ1).
+  { rewrite -hl0; by eapply length_subtype_targs_v1. }
+  apply list_lookup_fmap_inv in h as [c [-> hc]].
+  rewrite /Δsdt /= /SDT /= in hc.
+  rewrite lookup_insert_Some in hadef.
+  destruct hadef as [[<- <-] | hadef]; simpl in *; first done.
+  destruct hadef as (? & h).
+  rewrite lookup_singleton_Some in h.
+  destruct h as [<- <-]; simpl in *.
+  inv hσ; simpl in *.
+  destruct i as [ | i]; simpl in *.
+  - case : hc => <- /=.
+    rewrite /subst_constraint /=.
+    apply SubConstraint; by set_solver.
+  - done.
+Qed.
+
+Lemma has_fields_C : has_fields "C" {[ "$prop" := (Private, BoolT, "C") ]}.
+Proof.
+  move => f vis fty orig; split => h.
+  - inv h.
+    + rewrite /pdefs /= lookup_insert in H.
+      simplify_eq.
+      rewrite /C /= lookup_singleton_Some in H0.
+      by destruct H0 as [<- <-].
+    + by rewrite /pdefs /= lookup_insert in H; simplify_eq.
+  - rewrite lookup_singleton_Some in h.
+    destruct h as [<- [= <- <- <-]].
+    change Private with (Private, BoolT).1.
+    by econstructor.
+Qed.
+
+Lemma has_fields_M : has_fields "M" ∅.
+Proof.
+  move => f vis fty orig; split => h.
+  - inv h.
+    + rewrite /pdefs /= lookup_insert_ne // lookup_insert in H.
+      by simplify_eq.
+    + by rewrite /pdefs /= lookup_insert_ne // lookup_insert in H; simplify_eq.
+  - done. 
+Qed.
+
+Lemma wf_extends_dyn : map_Forall wf_cdef_extends_dyn pdefs.
+Proof.
+  rewrite map_Forall_lookup => c0 d0.
+  rewrite lookup_insert_Some.
+  case => [[<- <-]|[?]]; first done.
+  rewrite lookup_insert_Some.
+  case => [[? <-]|[?]] //.
+Qed.
+
+Lemma has_method_C m o mdef:
+  has_method m "C" o mdef →
+  (m = "get" ∧ o = "C" ∧ mdef = Get_) ∨
+  (m = "breakit" ∧ o = "C" ∧ mdef = BreakIt) ∨
+  (m = "set" ∧ o = "C" ∧ mdef = Set_).
+Proof.
+  move => h; inv h; last first.
+  { rewrite lookup_insert in H.
+    by simplify_eq.
+  }
+  rewrite lookup_insert in H.
+  simplify_eq.
+  rewrite lookup_insert_Some in H0.
+  case: H0 => [[? <-]|[?]].
+  { by firstorder. }
+  rewrite lookup_insert_Some => h.
+  case: h => [[? <-]|[?]].
+  - firstorder.
+  - rewrite lookup_singleton_Some => h.
+    by firstorder.
+Qed.
+
+Lemma has_method_M m o mdef:
+  has_method m "M" o mdef →
+  (m = "main" ∧ o = "M" ∧ mdef = main_fun).
+Proof.
+  move => h; inv h.
+  - rewrite lookup_insert_ne // lookup_insert // in H.
+    simplify_eq.
+    rewrite lookup_singleton_Some in H0.
+    by firstorder.
+  - rewrite lookup_insert_ne // lookup_insert // in H.
+    by simplify_eq.
+Qed.
+
+Lemma wf_methods_dyn : map_Forall wf_cdef_methods_dyn_wf pdefs.
+Proof.
+  rewrite map_Forall_lookup => c0 d0.
+  rewrite lookup_insert_Some.
+  case => [[<- <-]|[?]].
+  { move => m o mdef hm.
+    apply has_method_C in hm as [(-> & -> & ->) | [(-> & -> & ->) | (-> & -> & ->)]].
+    - exists (gen_targs (length C.(generics))).
+      split; first by eauto.
+      by move => i c /=.
+    - exists (gen_targs (length C.(generics))).
+      split; first by eauto.
+      by move => i c /=.
+    - exists (gen_targs (length C.(generics))).
+      split; first by eauto.
+      by move => i c /=.
+  }
+  rewrite lookup_singleton_Some.
+  case => [<- <-].
+  move => m o mdef hm.
+  apply has_method_M in hm as (-> & -> & ->).
+  exists (gen_targs (length M.(generics))).
+  split; first by constructor.
+  move => i c /=.
+  rewrite list_lookup_singleton_Some.
+  case => ? <- /=.
+  constructor; by set_solver.
+Qed.
+
+Lemma wf_fields_dyn : map_Forall wf_cdef_fields_dyn_wf pdefs.
+Proof.
+  rewrite map_Forall_lookup => c0 d0.
+  rewrite lookup_insert_Some.
+  case => [[<- <-]|[?]].
+  { move => fields hf.
+    move : has_fields_C => hf0.
+    rewrite (has_fields_fun _ _ _  hf hf0).
+    by apply map_Forall_singleton.
+  }
+  rewrite lookup_singleton_Some.
+  case => [<- <-].
+  move => fields hf /=.
+  move : has_fields_M => hf0.
+  rewrite (has_fields_fun _ _ _  hf hf0).
+  by apply map_Forall_empty.
+Qed.
+
+Lemma wf_mdefs_dyn : map_Forall cdef_wf_mdef_dyn_ty pdefs.
+Proof.
+  rewrite map_Forall_lookup => c0 d0.
+  rewrite lookup_insert_Some.
+  case => [[<- <-]|[?]].
+  { move => k m hm.
+    rewrite lookup_insert_Some in hm.
+    case : hm => [[<- <-]|[?]] //.
+    { rewrite /C /= /SDT_M /CSDT /wf_mdef_dyn_ty /=.
+    pose (Γ := {|
+        type_of_this := ("C", []);
+        ctxt := to_dyn <$> {["$vi" := BoolT]};
+      |}
+      ).
+    assert (wf_lty Γ).
+    { split => //.
+      - rewrite /this_type /=.
+        by econstructor => //.
+      - rewrite /Γ /=.
+        apply map_Forall_lookup => i ty.
+        rewrite lookup_fmap fmap_Some => [[ty0]].
+        rewrite lookup_singleton_Some.
+        by case => [[? <-]] ->.
+    }
+    exists Γ; split; first done.
+    split.
+    - eapply SetPrivTy.
+      + done.
+      + by change Private with (Private, BoolT).1; eapply HasField.
+      + simpl.
+        econstructor.
+        rewrite /= /to_dyn /=.
+        rewrite lookup_fmap /=.
+        rewrite lookup_insert /=.
+        Search lookup "fmap".
+        rewrite map_Forall_lookup.
+        apply map_Forall_lookup => i ty //.
+      rewrite lookup_fmap fmap_Some => [[ty0]].
+      rewrite lookup_singleton_Some.
+      by case => [[? <-]] ->.
+    - apply ESubTy with NullT => //.
+      + by constructor.
+      + by constructor.
+      + apply SubTrans with SupportDynT; by eauto.
+  }
+  rewrite lookup_insert_Some.
+  case => [[<- <-]|[?]] //.
+  { move => k m hm.
+    rewrite lookup_insert_Some in hm.
+    case : hm => [[<- <-] | ].
+    - rewrite /wf_mdef_dyn_ty.
+      pose (Γ := {|
+        type_of_this := ("Box", gen_targs 1);
+        ctxt := to_dyn <$> {[ "$y" := GenT 0 ]};
+      |}
+      ).
+      assert (wf_lty Γ).
+      { split => //.
+        - rewrite /this_type /=.
+          econstructor => //.
+          by apply gen_targs_wf_2.
+        - rewrite /Γ /=.
+          apply map_Forall_lookup => i ty.
+          rewrite lookup_fmap fmap_Some => [[ty0]].
+          rewrite lookup_singleton_Some.
+          by case => [[? <-]] ->.
+      }
+      exists Γ; split; first done.
+      rewrite /BoxSet /= /SDT_M /= /BoxSetSDT /=.
+      split.
+      + eapply SetPrivTy => //.
+        * change Private with (Private, GenT 0).1.
+          by econstructor.
+        * apply ESubTy with DynamicT => //=.
+          { by constructor. }
+          { constructor. by lia. }
+          { by constructor. }
+          { apply SubConstraint.
+            by set_solver.
+          }
+      + apply ESubTy with NullT => //=.
+        * by constructor.
+        * by constructor.
+        * apply SubTrans with SupportDynT; by eauto.
+    - case => ?.
+      rewrite lookup_singleton_Some => [[<- <-]].
+      rewrite /wf_mdef_dyn_ty.
+      pose (Γ := {|
+        type_of_this := ("Box", gen_targs 1);
+        ctxt := {[ "$ret" := GenT 0 ]};
+      |}
+      ).
+      assert (wf_lty Γ).
+      { split => //.
+        - rewrite /this_type /=.
+          econstructor => //.
+          by apply gen_targs_wf_2.
+        - rewrite /Γ /=.
+          by apply map_Forall_singleton.
+      }
+      pose (Γ0 := {| type_of_this := ("Box", gen_targs 1); ctxt := to_dyn <$> ∅ |}).
+      exists Γ; split; first done.
+      rewrite /Get /= /SDT_M /= /BoxGetSDT /=.
+      split.
+      + replace Γ with (<[ "$ret" := subst_ty (gen_targs 1) (GenT 0)]> Γ0) ; last first.
+        { rewrite /Γ0 /Γ /= /local_tys_insert /=.
+          f_equal.
+          by rewrite fmap_empty insert_empty.
+        }
+        eapply GetPrivTy => //.
+        change Private with (Private, GenT 0).1.
+        by econstructor.
+      + apply ESubTy with (GenT 0) => //=.
+        * by constructor.
+        * by constructor.
+        * apply SubConstraint.
+          by set_solver.
+  }
+Qed.
+
+Lemma helper_ext: ∀ A B σ0, extends_using A B σ0 → A = "ROBox" ∧ B = "Box" ∧ σ0 = [GenT 0].
+Proof.
+  move => A B σ0 h; inv h.
+  rewrite /pdefs /= lookup_insert_Some in H.
+  destruct H as [[<- <-] | [? H]].
+  { split => //.
+    rewrite /ROBox /= in H0; by simplify_eq.
+  }
+  rewrite lookup_singleton_Some in H.
+  destruct H as [<- <-].
+  by rewrite /Box /= in H0.
+Qed.
+
+Lemma helper_in_Box : ∀ T σt, inherits_using "Box" T σt → T = "Box" ∧ σt = [GenT 0].
+Proof.
+  move => T σt h; inv h.
+  + rewrite /pdefs /=.
+    do 1 (rewrite lookup_insert_ne // in H).
+    rewrite lookup_insert in H.
+    by simplify_eq.
+  + apply helper_ext in H.
+    destruct H; discriminate.
+  + apply helper_ext in H.
+    destruct H; discriminate.
+Qed.
+
+Lemma helper_in_ROBox : ∀ T σt, inherits_using "ROBox" T σt →
+  (T = "ROBox" ∧ σt = [GenT 0]) ∨
+  (T = "Box" ∧ σt = [GenT 0]).
+Proof.
+  move => T σt h; inv h.
+  + rewrite /pdefs /=.
+    rewrite lookup_insert in H.
+    left.
+    by simplify_eq.
+  + apply helper_ext in H.
+    destruct H; right; by simplify_eq.
+  + apply helper_ext in H.
+    destruct H as [_ [-> ->]]; right.
+    apply helper_in_Box in H0 as [-> ->].
+    done.
+Qed.
+
+Lemma helper_in: ∀ A B σ0, inherits_using A B σ0 →
+     (A = "Box" ∧ B = "Box" ∧ σ0 = [GenT 0]) ∨
+     (A = "ROBox" ∧ B = "Box" ∧ σ0 = [GenT 0]) ∨
+     (A = "ROBox" ∧ B = "ROBox" ∧ σ0 = [GenT 0]).
+Proof.
+  move => A B σ0 h.
+  inv h.
+  + rewrite /pdefs /=.
+    rewrite lookup_insert_Some in H.
+    destruct H as [[<- <-]|[? H]].
+    { by right; right. }
+    rewrite lookup_singleton_Some in H.
+    case : H => <- <-.
+    by left.
+  + apply helper_ext in H as [-> [-> ->]].
+    by right; left.
+  + apply helper_ext in H as [-> [-> ->]].
+    apply helper_in_Box in H0 as [-> ->].
+    by right; left.
+Qed.
+
+Lemma wf_override : wf_method_override pdefs.
+Proof.
+  move => A B adef bdef m σ0 mA mB hA hB hin hmA hmB.
+  apply helper_in in hin.
+  destruct hin as [[-> [-> ->]] | hin].
+  { rewrite /pdefs /= in hA, hB.
+    rewrite lookup_insert_ne // in hA.
+    rewrite lookup_insert_ne // in hB.
+    rewrite !lookup_insert in hA, hB.
+    simplify_eq.
+    change [GenT 0] with (gen_targs 1).
+    rewrite /Box /= in hmA.
+    rewrite lookup_insert_Some in hmA.
+    case: hmA => [[? <-] | ].
+    - rewrite /Box /BoxSet /=.
+      rewrite subst_mdef_gen_targs; first by apply mdef_incl_reflexive.
+      split => /=.
+      { apply map_Forall_singleton.
+        by repeat constructor.
+      }
+      split; first by constructor.
+      split; first by repeat constructor.
+      by repeat constructor.
+    - case => ?.
+      rewrite lookup_singleton_Some => [[? <-]].
+      rewrite /= subst_mdef_gen_targs; first by apply mdef_incl_reflexive.
+      split => /=; first by apply map_Forall_empty.
+      split; first by repeat constructor.
+      split; first by repeat constructor.
+      by repeat constructor.
+  }
+  destruct hin as [[-> [-> ->]] | hin].
+  { rewrite /pdefs /= in hA, hB.
+    rewrite lookup_insert in hA.
+    rewrite  lookup_insert_ne // lookup_insert in hB.
+    simplify_eq.
+    rewrite /ROBox /= lookup_singleton_Some in hmA.
+    destruct hmA as [<- <-].
+    rewrite /Box /= lookup_insert in hmB.
+    simplify_eq.
+    rewrite /ROBox /ROBoxSet /BoxSet /=.
+    split; last split => /=.
+    - by set_solver.
+    - move => k A B.
+      rewrite lookup_singleton_Some => [[<- <-]] /=.
+      rewrite lookup_fmap lookup_insert /= => [[<-]].
+      by eauto.
+    - by eauto.
+  }
+  destruct hin as [-> [-> ->]].
+  rewrite /pdefs /= in hA, hB.
+  rewrite !lookup_insert in hA, hB.
+  simplify_eq.
+  change [GenT 0] with (gen_targs 1).
+  rewrite /ROBox /= in hmA.
+  rewrite lookup_insert_Some in hmA.
+  case: hmA => [[? <-] | ].
+  - rewrite /ROBoxSet /=.
+    rewrite subst_mdef_gen_targs; first by apply mdef_incl_reflexive.
+    split => /=.
+    { apply map_Forall_singleton.
+      by repeat constructor.
+    }
+    split; first by constructor.
+    split; first by repeat constructor.
+    by repeat constructor.
+  - case => ?.
+    by rewrite lookup_empty.
+Qed.
+
+Lemma wf_parent : map_Forall (λ _cname, wf_cdef_parent pdefs) pdefs.
+Proof.
+  apply map_Forall_lookup => c0 d0.
+  rewrite lookup_insert_Some.
+  case => [[? <-] | [?]].
+  { split.
+    + econstructor => //.
+      by repeat constructor.
+    + by repeat constructor.
+  }
+  rewrite lookup_insert_Some.
+  by case => [[? <-] | [?]].
+Qed.
+
+Lemma wf_fields : map_Forall (λ _cname, wf_cdef_fields) pdefs.
+Proof.
+  rewrite map_Forall_lookup => c0 d0.
+  rewrite lookup_insert_Some.
+  case => [[? <-]|[?]].
+  { by rewrite /wf_cdef_fields /ROBox. }
+  rewrite lookup_singleton_Some.
+  case => [? <-].
+  by rewrite /wf_cdef_fields /Box.
+Qed.
+
+Lemma wf_fields_bounded : map_Forall (λ _cname, wf_cdef_fields_bounded) pdefs.
+Proof.
+  rewrite map_Forall_lookup => c0 d0.
+  rewrite lookup_insert_Some.
+  case => [[? <-]|[?]].
+  { by apply map_Forall_empty. }
+  rewrite lookup_singleton_Some.
+  case => [? <-].
+  apply map_Forall_singleton.
+  by repeat constructor.
+Qed.
+
+Lemma wf_fields_wf  : map_Forall (λ _cname, wf_cdef_fields_wf) pdefs.
+Proof.
+  rewrite map_Forall_lookup => c0 d0.
+  rewrite lookup_insert_Some.
+  case => [[? <-]|[?]].
+  { by apply map_Forall_empty. }
+  rewrite lookup_singleton_Some.
+  case => [? <-].
+  apply map_Forall_singleton.
+  by repeat constructor.
+Qed.
+
+Lemma wf_fields_mono : map_Forall (λ _cname, wf_field_mono) pdefs.
+Proof.
+  rewrite map_Forall_lookup => c0 d0.
+  rewrite lookup_insert_Some.
+  case => [[? <-]|[?]].
+  { by apply map_Forall_empty. }
+  rewrite lookup_singleton_Some.
+  case => [? <-].
+  apply map_Forall_singleton.
+  by repeat constructor.
+Qed.
+
+Lemma wf_methods_bounded : map_Forall (λ _cname, cdef_methods_bounded) pdefs.
+Proof.
+  rewrite map_Forall_lookup => c0 d0.
+  rewrite lookup_insert_Some.
+  case => [[? <-]|[?]].
+  { rewrite /cdef_methods_bounded /ROBox /=.
+    apply map_Forall_singleton.
+    split.
+    { apply map_Forall_singleton.
+      by repeat constructor.
+    }
+    split; by repeat constructor.
+  }
+  rewrite lookup_singleton_Some => [[? <-]].
+  apply map_Forall_lookup => m mdef.
+  rewrite /Box /= lookup_insert_Some => [[[? <-] | ]].
+  - split.
+    { apply map_Forall_singleton.
+      by repeat constructor.
+    }
+    split; by repeat constructor.
+  - case => ?.
+    rewrite lookup_singleton_Some => [[? <-]].
+    split; first by apply map_Forall_empty.
+    by repeat constructor.
+Qed.
+
+Lemma wf_methods_wf : map_Forall (λ _cname, wf_cdef_methods_wf) pdefs.
+Proof.
+  rewrite map_Forall_lookup => c0 d0.
+  rewrite lookup_insert_Some.
+  case => [[? <-]|[?]].
+  { rewrite /cdef_methods_bounded /ROBox /=.
+    apply map_Forall_singleton.
+    split.
+    { apply map_Forall_singleton.
+      by repeat constructor.
+    }
+    by repeat constructor.
+  }
+  rewrite lookup_singleton_Some => [[? <-]].
+  apply map_Forall_lookup => m mdef.
+  rewrite /Box /= lookup_insert_Some => [[[? <-] | ]].
+  - split.
+    { apply map_Forall_singleton.
+      by repeat constructor.
+    }
+    by repeat constructor.
+  - case => ?.
+    rewrite lookup_singleton_Some => [[? <-]].
+    split; first by apply map_Forall_empty.
+    by repeat constructor.
+Qed.
+
+Lemma wf_methods_mono : map_Forall (λ _cname, wf_cdef_methods_mono) pdefs.
+Proof.
+  rewrite map_Forall_lookup => c0 d0.
+  rewrite lookup_insert_Some.
+  case => [[? <-]|[?]].
+  { rewrite /cdef_methods_bounded /ROBox /=.
+    apply map_Forall_singleton.
+    split.
+    { apply map_Forall_singleton.
+      by repeat constructor.
+    }
+    by repeat constructor.
+  }
+  rewrite lookup_singleton_Some => [[? <-]].
+  apply map_Forall_lookup => m mdef.
+  rewrite /Box /= lookup_insert_Some => [[[? <-] | ]].
+  - split.
+    { apply map_Forall_singleton.
+      by repeat constructor.
+    }
+    by repeat constructor.
+  - case => ?.
+    rewrite lookup_singleton_Some => [[? <-]].
+    split; first by apply map_Forall_empty.
+    by repeat constructor.
+Qed.
+
+Lemma wf_mdefs : map_Forall cdef_wf_mdef_ty pdefs.
+Proof.
+  rewrite map_Forall_lookup => c0 d0.
+  rewrite lookup_insert_Some.
+  case => [[<- <-]|[?]].
+  { move => k m hm.
+    rewrite lookup_singleton_Some in hm.
+    case : hm => ? <-.
+    rewrite /ROBox /= /ROBoxSet /wf_mdef_dyn_ty /=.
+    pose (Γ := {|
+        type_of_this := ("ROBox", gen_targs 1);
+        ctxt := {["$y" := MixedT]};
+      |}
+      ).
+    assert (wf_lty Γ).
+    { split => //.
+      - rewrite /this_type /=.
+        econstructor => //.
+        by apply gen_targs_wf_2.
+      - rewrite /Γ /=.
+        by apply map_Forall_singleton.
+    }
+    exists Γ; split; first done.
+    split.
+    - constructor => //.
+      constructor; first by repeat constructor.
+      by apply map_Forall_singleton.
+    - by constructor.
+  }
+  rewrite lookup_insert_Some.
+  case => [[<- <-]|[?]] //.
+  { move => k m hm.
+    rewrite lookup_insert_Some in hm.
+    case : hm => [[? <-] | ].
+    - rewrite /wf_mdef_dyn_ty.
+      pose (Γ := {|
+        type_of_this := ("Box", gen_targs 1);
+        ctxt := {[ "$y" := GenT 0 ]};
+      |}
+      ).
+      assert (wf_lty Γ).
+      { split => //.
+        - rewrite /this_type /=.
+          econstructor => //.
+          by apply gen_targs_wf_2.
+        - rewrite /Γ /=.
+          by apply map_Forall_singleton.
+      }
+      exists Γ; split; first done.
+      rewrite /BoxSet /= /BoxSetSDT /=.
+      split.
+      + eapply SetPrivTy => //.
+        * change Private with (Private, GenT 0).1.
+          by econstructor.
+        * by constructor.
+      + by constructor.
+    - case => ?.
+      rewrite lookup_singleton_Some => [[? <-]].
+      rewrite /wf_mdef_dyn_ty.
+      pose (Γ := {|
+        type_of_this := ("Box", gen_targs 1);
+        ctxt := {[ "$ret" := GenT 0 ]};
+      |}
+      ).
+      assert (wf_lty Γ).
+      { split => //.
+        - rewrite /this_type /=.
+          econstructor => //.
+          by apply gen_targs_wf_2.
+        - rewrite /Γ /=.
+          by apply map_Forall_singleton.
+      }
+      pose (Γ0 := {| type_of_this := ("Box", gen_targs 1); ctxt := ∅ |}).
+      exists Γ; split; first done.
+      rewrite /Get /= /BoxGetSDT /=.
+      split.
+      + replace Γ with (<[ "$ret" := subst_ty (gen_targs 1) (GenT 0)]> Γ0) ; last first.
+        { rewrite /Γ0 /Γ /= /local_tys_insert /=.
+          by f_equal.
+        }
+        eapply GetPrivTy => //.
+        change Private with (Private, GenT 0).1.
+        by econstructor.
+      + by constructor.
+  }
+Qed.
+
+Lemma wf_mono : map_Forall (λ _cname, wf_cdef_mono) pdefs.
+Proof.
+  rewrite map_Forall_lookup => x cx.
+  rewrite lookup_insert_Some.
+  case => [[? <-]|[?]].
+  { rewrite /wf_cdef_mono /ROBox /=.
+    econstructor => //.
+    + move => i wi ti //=.
+      rewrite list_lookup_singleton_Some.
+      case => [-> <-].
+      simpl.
+      case => <- _.
+      by constructor.
+    + move => i wi ti //=.
+      rewrite list_lookup_singleton_Some.
+      case => [-> <-].
+      simpl.
+      case => <- _.
+      by constructor.
+  }
+  rewrite lookup_singleton_Some.
+  by case => [? <-].
+Qed.
+
+Lemma wf_constraints_wf : map_Forall (λ _cname, wf_cdef_constraints_wf) pdefs.
+Proof.
+  rewrite map_Forall_lookup => c0 d0.
+  rewrite lookup_insert_Some.
+  case => [[? <-]|[?]].
+  { by rewrite /wf_cdef_constraints_wf /ROBox /= Forall_nil. }
+  rewrite lookup_singleton_Some => [[? <-]].
+  { by rewrite /wf_cdef_constraints_wf /Box /= Forall_nil. }
+Qed.
+
+Lemma wf_constraints_bounded : map_Forall (λ _cname, wf_cdef_constraints_bounded) pdefs.
+Proof.
+  rewrite map_Forall_lookup => c0 d0.
+  rewrite lookup_insert_Some.
+  case => [[? <-]|[?]].
+  { by rewrite /wf_cdef_constraints_bounded /ROBox /= Forall_nil. }
+  rewrite lookup_singleton_Some => [[? <-]].
+  { by rewrite /wf_cdef_constraints_bounded /Box /= Forall_nil. }
+Qed.
+
+Lemma wf_parent_ok : map_Forall (λ _cname, wf_cdef_parent_ok) pdefs.
+Proof.
+  rewrite map_Forall_lookup => c0 d0.
+  rewrite lookup_insert_Some.
+  case => [[? <-]|[?]].
+  { rewrite /wf_cdef_parent_ok /=.
+    econstructor => // i ty.
+    rewrite list_lookup_singleton_Some => [[? <-]].
+    by constructor.
+  }
+  rewrite lookup_singleton_Some.
+  case => [? <-].
+  by rewrite /wf_cdef_parent_ok.
+Qed.
+
+Lemma wf_constraints_ok : map_Forall (λ _cname, wf_cdef_constraints_ok) pdefs.
+Proof.
+  rewrite map_Forall_lookup => c0 d0.
+  rewrite lookup_insert_Some.
+  case => [[? <-]|[?]].
+  {  rewrite /wf_cdef_constraints_ok /ROBox /=.
+    by constructor.
+  }
+  rewrite lookup_singleton_Some => [[? <-]].
+  { rewrite /wf_cdef_constraints_ok /Box /=.
+    by constructor.
+  }
+Qed.
+
+Lemma wf_methods_ok : map_Forall (λ _cname, cdef_methods_ok) pdefs.
+Proof.
+  rewrite map_Forall_lookup => c0 d0.
+  rewrite lookup_insert_Some.
+  case => [[? <-]|[?]].
+  { rewrite /cdef_methods_ok /ROBox /=.
+    apply map_Forall_singleton.
+    rewrite /mdef_ok /=.
+    split; last by constructor.
+    apply map_Forall_singleton.
+    by constructor.
+  }
+  rewrite lookup_singleton_Some => [[? <-]].
+  rewrite /cdef_methods_ok /Box /=.
+  rewrite map_Forall_lookup => x mx.
+  rewrite lookup_insert_Some.
+  case => [[? <-]|[?]].
+  * rewrite /mdef_ok /BoxSet /=.
+    split; last by constructor.
+    apply map_Forall_singleton.
+    by constructor.
+  * rewrite lookup_singleton_Some => [[? <-]].
+    rewrite /mdef_ok /Get /=.
+    split; first by apply map_Forall_empty.
+    by constructor.
+Qed.
+
+Lemma wf: wf_cdefs pdefs.
+Proof.
+  split.
+  by apply wf_parent.
+  by apply wf_parent_ok.
+  by apply wf_constraints_wf.
+  by apply wf_constraints_ok.
+  by apply wf_constraints_bounded.
+  by apply wf_override.
+  by apply wf_fields.
+  by apply wf_fields_bounded.
+  by apply wf_fields_wf.
+  by apply wf_fields_mono.
+  by apply wf_methods_bounded.
+  by apply wf_methods_wf.
+  by apply wf_methods_mono.
+  by apply wf_methods_ok.
+  by apply wf_mdefs.
+  by apply wf_mono.
+  by apply wf_extends_dyn.
+  by apply wf_methods_dyn.
+  by apply wf_fields_dyn.
+  by apply wf_mdefs_dyn.
+Qed.
